before removing comments

src/Distributions/DiscreteLaplace/Equivalence.dfy
@@ -28,7 +28,7 @@ module DiscreteLaplace.Equivalence {
         var (u, s) :- Uniform.Model.Sample(scale.numer)(s);
         var (d, s) :- BernoulliExpNeg.Model.Sample(Rationals.Rational(u, scale.numer))(s);
         if d then
-          var (v, s) :- SampleTailRecursiveHelper()(s);
+          var (v, s) :- SampleTailRecursiveHelper(s);
           var x := u + scale.numer * v;
           var y := x / scale.denom;
           var sample := Coin.Model.Sample(s);
@@ -37,25 +37,30 @@ module DiscreteLaplace.Equivalence {
           SampleTailRecursive(scale, b, y)(s)
   }
 
-  ghost function SampleTailRecursiveHelper(): Monad.Hurd<int> 
-    requires Loops.WhileCutTerminates(Model.SampleHelperLoopCondition, Model.SampleHelperLoopBody, (true, 0), s)   
+  ghost function SampleTailRecursiveHelper(s: Rand.Bitstream): Monad.Result<int>
+    requires Loops.WhileCutTerminates(Model.SampleHelperLoopCondition, Model.SampleHelperLoopBody, (true, 0), s)
   {
     var f := (x: (bool, int)) => x.1;
-    Monad.Map(SampleTailRecursiveHelperLoop(), f)
+    SampleTailRecursiveHelperLoop(s).Map(f)
   }
 
-  ghost function SampleTailRecursiveHelperLoop(x: (bool, int) := (true, 0)): Monad.Hurd<(bool, int)> 
-    requires Loops.WhileCutTerminates(Model.SampleHelperLoopCondition, Model.SampleHelperLoopBody, x, s) 
+  ghost function SampleTailRecursiveHelperLoop(s: Rand.Bitstream, x: (bool, int) := (true, 0)): Monad.Result<(bool, int)>
+    requires Loops.WhileCutTerminates(Model.SampleHelperLoopCondition, Model.SampleHelperLoopBody, x, s)
   {
     var fuel := Loops.LeastFuel(Model.SampleHelperLoopCondition, Model.SampleHelperLoopBody, x, s);
-    SampleTailRecursiveHelperLoopCut(x, fuel)
+    SampleTailRecursiveHelperLoopCut(x, fuel)(s)
   }
 
-  ghost function SampleTailRecursiveHelperLoopCut(x: (bool, int) := (true, 0), fuel): Monad.Hurd<(bool, int)> {
-    if fuel == 0 || !x.0 then 
-      Monad.Return(x)
-    else
-      Monad.Bind(Model.SamplerHelperLoopBody(x), (x': (bool, int)) => SampleTailRecursiveHelperLoop(x', fuel - 1))
+  ghost function SampleTailRecursiveHelperLoopCut(x: (bool, int) := (true, 0), fuel: nat): Monad.Hurd<(bool, int)>
+    decreases fuel
+  {
+    (s: Rand.Bitstream) => 
+      if fuel == 0 || !x.0 then
+        Monad.Result(x, s)
+      else
+        var (a, s') :- BernoulliExpNeg.Model.Sample(Rationals.Int(1))(s);
+        SampleTailRecursiveHelperLoopCut((a, if a then x.1 + 1 else x.1), fuel - 1)(s')
+        // Monad.Bind(Model.SampleHelperLoopBody(x), (x': (bool, int)) => SampleTailRecursiveHelperLoopCut(x', fuel - 1))
   }
 
   /*******
@@ -67,65 +72,76 @@ module DiscreteLaplace.Equivalence {
     ensures SampleTailRecursive(scale)(s) == Model.Sample(scale)(s)
 
   lemma SampleTailRecursiveHelperEquivalence(s: Rand.Bitstream)
-    ensures SampleTailRecursiveHelper()(s) == Model.SampleHelper()(s)
+    requires Loops.WhileCutTerminates(Model.SampleHelperLoopCondition, Model.SampleHelperLoopBody, (true, 0), s)
+    ensures SampleTailRecursiveHelper(s) == Model.SampleHelper(s)
   {
     var f := (x: (bool, int)) => x.1;
-    var (x, s') :- SampleTailRecursiveHelperLoop((true, 0))(s);
-    var (x', s'') :- Model.SampleHelperLoop((true, 0))(s);
+
     calc {
-      SampleTailRecursiveHelper()(s);
-      Monad.Map(SampleTailRecursiveHelperLoop(), f)(s);
-      Monad.Bind(SampleTailRecursiveHelperLoop(), (x: bool, int) => Monad.Return(f(x)))(s);
-      Monad.Return(f(x'))(s');
-      { assert x == x' && s' == s'' by { SampleTailRecursiveHelperCutEquivalence((ture, 0), s) }; }
-      Monad.Return(f(x''))(s'');
-      Monad.Bind(Model.SampleHelperLoop(), (x: bool, int) => Monad.Return(f(x)));
-      Monad.Map(Model.SampleHelperLoop(), f)(s);
-      Model.SampleHelper()(s);
+      SampleTailRecursiveHelper(s);
+      SampleTailRecursiveHelperLoop(s).Map(f);
+      if SampleTailRecursiveHelperLoop(s).Diverging? then Monad.Diverging else Monad.Result(f(SampleTailRecursiveHelperLoop(s).value), SampleTailRecursiveHelperLoop(s).rest);
+      { SampleTailRecursiveHelperEquivalence2((true, 0), s); }
+      if Model.SampleHelperLoop(s).Diverging? then Monad.Diverging else Monad.Result(f(Model.SampleHelperLoop(s).value), Model.SampleHelperLoop(s).rest);
+      Model.SampleHelperLoop(s).Map(f);
+      Model.SampleHelper(s);
     }
   }
 
-  lemma SampleTailRecursiveHelperCutEquivalence(x: (bool, int), s: Rand.Bitstream)
-    requires Loops.WhileCutTerminates(Model.SampleHelperLoopCondition, Model.SampleHelperLoopBody, x, s) 
-    ensures SampleTailRecursiveHelperLoop(x)(s) == Model.SampleHelperLoop(x)(s)
+  lemma SampleTailRecursiveHelperEquivalence2(x: (bool, int), s: Rand.Bitstream)
+    requires Loops.WhileCutTerminates(Model.SampleHelperLoopCondition, Model.SampleHelperLoopBody, x, s)
+    ensures SampleTailRecursiveHelperLoop(s, x) == Model.SampleHelperLoop(s, x)
   {
     var fuel := Loops.LeastFuel(Model.SampleHelperLoopCondition, Model.SampleHelperLoopBody, x, s);
     calc {
-      SampleTailRecursiveHelperLoop(x)(s);
+      SampleTailRecursiveHelperLoop(s, x);
       SampleTailRecursiveHelperLoopCut(x, fuel)(s);
-      { SampleTailRecursiveHelperCutEquivalence(x, s, fuel); }
-      Loops.WhileCut(SampleHelperLoopCondition, SampleHelperLoopBody, x, fuel)(s);
-      Loops.While(SampleHelperLoopCondition, SampleHelperLoopBody)(x)(s);
-      Model.SampleHelperLoop(x)(s);
+      { SampleTailRecursiveHelperEquivalence3(x, s, fuel); }
+      Loops.WhileCut(Model.SampleHelperLoopCondition, Model.SampleHelperLoopBody, x, fuel)(s);
+      { reveal Loops.While(); }
+      Loops.While(Model.SampleHelperLoopCondition, Model.SampleHelperLoopBody)(x)(s);
+      Model.SampleHelperLoop(s, x);
     }
   }
 
-  lemma SampleTailRecursiveHelperCutEquivalence(x: (bool, int), s: Rand.Bitstream, fuel: nat)
-    ensures SampleTailRecursiveHelperLoopCut(x, fuel)(s) == Loops.WhileCut(SampleHelperLoopCondition, SampleHelperLoopBody, x, fuel)(s)
+  lemma SampleTailRecursiveHelperEquivalence3(x: (bool, int), s: Rand.Bitstream, fuel: nat)
+    decreases fuel
+    ensures SampleTailRecursiveHelperLoopCut(x, fuel)(s) == Loops.WhileCut(Model.SampleHelperLoopCondition, Model.SampleHelperLoopBody, x, fuel)(s)
   {
     if !x.0 {
       calc {
-        SampleTailRecursiveHelperLoopCut(x, fuel)(s)
+        SampleTailRecursiveHelperLoopCut(x, fuel)(s);
         Monad.Return(x)(s);
-        Loops.WhileCut(SampleHelperLoopCondition, SampleHelperLoopBody, x, fuel)(s);
+        Loops.WhileCut(Model.SampleHelperLoopCondition, Model.SampleHelperLoopBody, x, fuel)(s);
       }
     } else if fuel == 0 {
       calc {
-        SampleTailRecursiveHelperLoopCut(x, fuel)(s)
+        SampleTailRecursiveHelperLoopCut(x, fuel)(s);
         Monad.Return(x)(s);
-        Loops.WhileCut(SampleHelperLoopCondition, SampleHelperLoopBody, x, fuel)(s)
+        Loops.WhileCut(Model.SampleHelperLoopCondition, Model.SampleHelperLoopBody, x, fuel)(s);
       }
     } else {
-      var (x', s') :- Model.SamplerHelperLoopBody(x)(s);
-      calc {
-        SampleTailRecursiveHelperLoopCut(x, fuel)(s);
-        Monad.Bind(Model.SamplerHelperLoopBody(x), (x': (bool, int)) => SampleTailRecursiveHelperLoopCut(x', fuel - 1))(s);
-        SampleTailRecursiveHelperLoopCut(x', fuel - 1)(s');
-        { SampleTailRecursiveHelperEquivalence(x', s', fuel - 1); }
-        Loops.WhileCut(SampleHelperLoopCondition, SampleHelperLoopBody, x', fuel - 1)(s');
-        Monad.Bind(Model.SampleHelperLoopBody(x), (x': (bool, int) => Loops.WhileCut(SampleHelperLoopCondition, SampleHelperLoopBody, x', fuel - 1)))(s);
-        Monad.Bind(Model.SampleHelperLoopBody(x), (x': (bool, int) => Loops.WhileCut(SampleHelperLoopCondition, SampleHelperLoopBody, x', fuel - 1)))(s);
-        Loops.WhileCut(SampleHelperLoopCondition, SampleHelperLoopBody, x, fuel)(s)
+      var r := Model.SampleHelperLoopBody(x)(s);
+      if r.Result? {
+        var (x', s') := Model.SampleHelperLoopBody(x)(s).Extract();
+        calc {
+          SampleTailRecursiveHelperLoopCut(x, fuel)(s);
+          Monad.Bind(Model.SampleHelperLoopBody(x), (x': (bool, int)) => SampleTailRecursiveHelperLoopCut(x', fuel - 1))(s);
+          SampleTailRecursiveHelperLoopCut(x', fuel - 1)(s');
+          { SampleTailRecursiveHelperEquivalence3(x', s', fuel - 1); }
+          Loops.WhileCut(Model.SampleHelperLoopCondition, Model.SampleHelperLoopBody, x', fuel - 1)(s');
+          Monad.Bind(Model.SampleHelperLoopBody(x), (x': (bool, int)) => Loops.WhileCut(Model.SampleHelperLoopCondition, Model.SampleHelperLoopBody, x', fuel - 1))(s);
+          Loops.WhileCut(Model.SampleHelperLoopCondition, Model.SampleHelperLoopBody, x, fuel)(s);
+        }
+      } else {
+        calc {
+          SampleTailRecursiveHelperLoopCut(x, fuel)(s);
+          Monad.Bind(Model.SampleHelperLoopBody(x), (x': (bool, int)) => SampleTailRecursiveHelperLoopCut(x', fuel - 1))(s);
+          Monad.Diverging;
+          Monad.Bind(Model.SampleHelperLoopBody(x), (x': (bool, int)) => Loops.WhileCut(Model.SampleHelperLoopCondition, Model.SampleHelperLoopBody, x', fuel - 1))(s);
+          Loops.WhileCut(Model.SampleHelperLoopCondition, Model.SampleHelperLoopBody, x, fuel)(s);
+        }
+      }
     }
   }
 }
