src/Distributions/DiscreteLaplace/Implementation.dfy
@@ -13,6 +13,7 @@ module DiscreteLaplace.Implementation {
   import Bernoulli
   import Coin
   import Equivalence
+  import Loops
 
   trait {:termination false} Trait extends Interface.Trait {
 
@@ -31,16 +32,7 @@ module DiscreteLaplace.Implementation {
         var u := UniformSample(scale.numer);
         var d := BernoulliExpNegSample(Rationals.Rational(u, scale.numer));
         if d {
-          var a := true;
-          var v := 0;
-          while a
-            decreases *
-          {
-            a := BernoulliExpNegSample(Rationals.Int(1));
-            if a {
-              v := v + 1;
-            }
-          }
+          var v := DiscreteLaplaceSampleHelper();
           var x := u + scale.numer * v;
           y := x / scale.denom;
           b := CoinSample();
@@ -51,5 +43,71 @@ module DiscreteLaplace.Implementation {
       Equivalence.SampleTailRecursiveEquivalence(scale, old(s));
     }
 
+    method DiscreteLaplaceSampleHelper() returns (v: int) 
+      modifies this
+      decreases *
+      ensures Model.SampleHelper.requires(old(s))
+      ensures Model.SampleHelper(old(s)) == Monad.Result(v, s)
+    {
+      assume {:axiom} Model.SampleHelper.requires(old(s));
+
+      var a := true;
+      v := 0;
+      ghost var fuel := Loops.LeastFuel(Model.SampleHelperLoopCondition, Model.SampleHelperLoopBody, (true, 0), old(s));
+
+      ghost var prevFuel := fuel;
+      ghost var prevA := a;
+      ghost var prevV := v;
+      ghost var prevS := s;
+    
+
+      a := BernoulliExpNegSample(Rationals.Int(1));
+      if a {
+        v := v + 1;
+      }
+      fuel := fuel - 1;
+
+      while a
+        decreases *
+        invariant Equivalence.SampleTailRecursiveHelperLoop(old(s)) == Equivalence.SampleTailRecursiveHelperLoopCut((a, v), fuel)(s)
+        //invariant !a ==> Equivalence.SampleTailRecursiveHelperLoopCut((a, v), fuel)(s) == Monad.Result((a, v), s); 
+        //invariant Equivalence.SampleTailRecursiveHelperLoop(old(s)) == Equivalence.SampleTailRecursiveHelperLoopCut((prevA, prevV), prevFuel)(prevS)
+        //invariant Equivalence.SampleTailRecursiveHelperLoopCut((prevA, prevV), prevFuel)(prevS) == Equivalence.SampleTailRecursiveHelperLoopCut((a, v), fuel)(s)
+      {
+        assume {:axiom} fuel > 1;
+        prevFuel := fuel;
+        prevA := a;
+        prevV := v;
+        prevS := s;
+
+        a := BernoulliExpNegSample(Rationals.Int(1));
+        if a {
+          v := v + 1;
+        }
+        fuel := fuel - 1;
+      }
+
+      //assert A1: Equivalence.SampleTailRecursiveHelperLoopCut((a, v), fuel)(s) == Monad.Result((a, v), s);
+      //assert A2: Equivalence.SampleTailRecursiveHelperLoop(old(s)) == Equivalence.SampleTailRecursiveHelperLoopCut((prevA, prevV), prevFuel)(prevS);
+      //assert A3: Equivalence.SampleTailRecursiveHelperLoopCut((prevA, prevV), prevFuel)(prevS) == Equivalence.SampleTailRecursiveHelperLoopCut((a, v), fuel)(s);
+      var f := (x: (bool, int)) => x.1;
+
+
+
+      calc {
+        Model.SampleHelper(old(s));
+        { Equivalence.SampleTailRecursiveHelperEquivalence(old(s)); }
+        Equivalence.SampleTailRecursiveHelper(old(s));
+        Equivalence.SampleTailRecursiveHelperLoop(old(s)).Map(f);
+        //{ reveal A2; }
+       // Equivalence.SampleTailRecursiveHelperLoopCut((prevA, prevV), prevFuel)(prevS).Map(f);
+       // { reveal A3; }
+        Equivalence.SampleTailRecursiveHelperLoopCut((a, v), fuel)(s).Map(f);
+        //{ reveal A1; }
+        Monad.Result((a, v), s).Map(f);
+        Monad.Result(v, s); 
+      }
+      
+    }
   }
 }
